# Warm up: Exponential Functions

## 1. Calculate with powers

a) $3^n \times 9 = 3^{n+2}$ 

b) $\frac{\normalsize x\times 4}{\normalsize (2x)^2} = \frac{\normalsize x\times 2^2}{\normalsize x^2 \times 2^2} = \frac{\normalsize x}{\normalsize x^2} = x^{-1}$

c) $\frac{\normalsize 3^4 \times 3}{\normalsize 3^{-2}} = 3^7$

d) $(a^2)^4 \times a^{-3} = a^5$

## 2. Solve inequations

a) 
$$2x+4 > 0$$
$$2x > -4$$
$$x > -2$$

b) 
$$x^2 - 1 < 0$$
$$x^2 < 1$$
$$x < 1$$

c) 
$$-3x + 4 \le 0$$
$$-3w \le -4$$
$$x \le \frac{4}{3}$$

d) 
$$x+4 > 3x + 1$$
$$2x > -3$$
$$x > \frac{-3}{2}$$

e) 
$$x^2 - 4 < - 5$$
$$x^2 > - 1$$
$$x > \emptyset$$

f)
$$-7x+1 > -3(x+1)$$
$$-7x+1 > -3x+3$$
$$-4x > -4$$
$$x > 1$$

## 3. Factorize

a) $3x-x^3 = x(3-x^2)$

b) $9-x^2 = (3-x)^2$

c) $5(x+1) + x^2(-x-1) = 5x+5 - x^3 - x^2 = 5x+5 = 5(x+1)$

d) $4x^2 - 4x + 1 = 4x(x-1+\frac{1}{4x})$

## 4. Derivate

## 5. Tangent

Derivate of $f(x) = x^2 - 2x + 3$ is $f'(x) = 2x-2$

1. $f'(2) = 2$
    
    $y=2(x-2)+3$
    
2. $f'(1) = 0$

    $y = 2$

## 6. Work with geometrical sequences
1. $u_n = 3 \times 2^n$ is geometrical because it's initial term is $3$ and it's common ratio is $3$

2. $(u_n)$ $q=\frac{1}{4}$ $u_0 = 2$

$$u_{n+1} = \frac{n}{4}$$

$$S = \sum_{k=0}^{k=10} u_k$$

$$S = u_0 + u_1 + ... + u_{10}$$

$$S = \frac{2}{1} + \frac{2}{4} + \frac{2}{16} + \frac{2}{64} + ... + \frac{2}{4^{10}}$$

$$S = 2 \times 4^0 + 2 \times 4^{-1} + 2 \times 4^{-2} + ... + 2 \times 4^{-10}$$

$$S = 2 \times (4^0 + 4^{-1} + 4^{-2} + ... + 4^{-10})$$

$$S = 2 \times 1.3333330154 = 2.6666660308$$

## 7. Evolution and geometrical sequence
a) $q = \frac{1}{3}$

b) $q = 1.10$

c) $q = 0.87$

d) $q = \frac{1}{4}$